add isabelle make_coupon_good proof

wasm-proofs/Wasm-Proof/isabelle_coupon.thy
@@ -2,120 +2,1077 @@ theory isabelle_coupon
   imports coupon
 begin
 
-fun make_storage_coupon_raw :: "handle list \<Rightarrow> handle \<Rightarrow> handle \<Rightarrow> handle option" where
-  "make_storage_coupon_raw (c # xs) l r =
-   (if (is_storage_coupon_api c) 
-    then (case (get_coupon_lhs c, get_coupon_rhs c) of
-     (Some l', Some r') \<Rightarrow> (if ( is_equal l l' \<and> is_equal r r') then Some (create_eq_coupon l r)
-                                                                else None)
-    | _ \<Rightarrow> None)
-    else None)"
-| "make_storage_coupon_raw [] l r = None"
+datatype coupon_type =
+  Force | Storage | Apply | Slice | Think | Eval | Eq
 
-fun make_tree_coupon_raw :: "handle list \<Rightarrow> handle \<Rightarrow> handle \<Rightarrow> handle option" where
-  "make_tree_coupon_raw coupons l r =
-   (if (\<forall>i. (i < length coupons \<longrightarrow> is_eq_coupon_api (coupons ! i))) then
+record coupon = 
+  type :: coupon_type
+  lhs :: handle
+  rhs :: handle
+
+consts
+  (* coupon-related ones *)
+  is_coupon :: "handle \<Rightarrow> bool"
+  create_coupon :: "coupon_type \<Rightarrow> handle \<Rightarrow> handle \<Rightarrow> handle"
+
+  get_coupon_lhs :: "handle \<Rightarrow> handle option"
+  get_coupon_rhs :: "handle \<Rightarrow> handle option"
+  get_coupon_type :: "handle \<Rightarrow> coupon_type option"
+
+  (* typeless Fix apis *)
+  get_tree_size_api :: "handle \<Rightarrow>  nat option"
+  get_tree_data_api :: "handle \<Rightarrow> nat \<Rightarrow> handle option"
+  create_application_thunk_api :: "handle \<Rightarrow> handle option"
+  create_selection_thunk_api :: "handle \<Rightarrow> handle option"
+  create_identification_thunk_api :: "handle \<Rightarrow> handle option"
+  create_strict_encode_api :: "handle \<Rightarrow> handle option"
+  create_shallow_encode_api :: "handle \<Rightarrow> handle option"
+
+  is_equal :: "handle \<Rightarrow>  handle \<Rightarrow> bool"
+
+(* coupon-related ones *)
+axiomatization where
+  get_coupon_lhs_match[simp]:
+  "get_coupon_lhs (create_coupon r x y) = Some x"
+and
+  get_coupon_rhs_match[simp]:
+  "get_coupon_rhs (create_coupon r x y) = Some y"
+and
+  get_coupon_type_match[simp]:
+  "get_coupon_type (create_coupon r x y) = Some r"
+and
+  get_coupon_type_exists[simp]:
+  "get_coupon_type c = Some t \<Longrightarrow> \<exists>r x y. c = create_coupon r x y"
+  
+(* typeless Fix api axioms *)
+axiomatization where
+  get_tree_data_api_match[simp]: 
+  "get_tree_data_api h i =
+    (case h of
+      (Data (Object (TreeObj t))) \<Rightarrow> 
+        (if i < length (get_tree_raw t) then 
+          Some (get_tree_data  t i) else None)
+    | _ \<Rightarrow> None)" 
+and
+  get_tree_size_api_match[simp]: 
+  "get_tree_size_api h =
+    (case h of
+      (Data (Object (TreeObj t))) \<Rightarrow> Some (get_tree_size t) 
+     | _ \<Rightarrow> None)" 
+and
+  create_application_thunk_api_match[simp]:
+  "create_application_thunk_api h =
+     (case h of
+       (Data (Object (TreeObj t))) \<Rightarrow> Some (Thunk (Application t))
+     | _ \<Rightarrow> None)"
+and
+  create_selection_thunk_api_match[simp]:
+  "create_selection_thunk_api h =
+   (case h of
+     (Data (Object (TreeObj t))) \<Rightarrow> Some (Thunk (Selection t))
+   | (Data (Ref (TreeRef t))) \<Rightarrow> Some (Thunk (Selection t))
+   | _ \<Rightarrow> None)"
+and
+  create_identification_thunk_api_match[simp]:
+  "create_identification_thunk_api h =
+   (case h of
+     (Data d) \<Rightarrow> Some (Thunk (Identification d))
+   | _ \<Rightarrow> None)"
+and
+  create_strict_encode_api_match[simp]:
+  "create_strict_encode_api h = 
+   (case h of
+     (Thunk th) \<Rightarrow> Some (Encode (Strict th))
+   | _ \<Rightarrow> None)"
+and
+  create_shallow_encode_api_match[simp]:
+  "create_shallow_encode_api h = 
+   (case h of
+     (Thunk th) \<Rightarrow> Some (Encode (Shallow th))
+   | _ \<Rightarrow> None)"
+and
+  is_equal_match [simp]:
+  "is_equal h1 h2 = (h1 = h2)"
+
+definition is_force_coupon :: "handle \<Rightarrow> bool" where
+  "is_force_coupon c \<equiv> (get_coupon_type c = Some Force)"
+
+definition is_storage_coupon :: "handle \<Rightarrow> bool" where
+  "is_storage_coupon c \<equiv> (get_coupon_type c = Some Storage)"
+
+definition is_apply_coupon :: "handle \<Rightarrow> bool" where
+  "is_apply_coupon c \<equiv> (get_coupon_type c = Some Apply)"
+
+definition is_slice_coupon :: "handle \<Rightarrow> bool" where
+  "is_slice_coupon c \<equiv> (get_coupon_type c = Some Slice)"
+
+definition is_think_coupon :: "handle \<Rightarrow> bool" where
+  "is_think_coupon c \<equiv> (get_coupon_type c = Some Think)"
+
+definition is_eq_coupon :: "handle \<Rightarrow> bool" where
+  "is_eq_coupon c \<equiv> (get_coupon_type c = Some Eq)"
+
+definition is_eval_coupon :: "handle \<Rightarrow> bool" where
+  "is_eval_coupon c \<equiv> (get_coupon_type c = Some Eval)"
+
+definition coupon_good :: "handle \<Rightarrow> bool"
+  where
+"coupon_good c = 
+  (case (get_coupon_type c, get_coupon_lhs c, get_coupon_rhs c) of 
+    (Some t, Some l, Some r) \<Rightarrow>
+      (case t of
+         Force \<Rightarrow> coupon_force l r
+       | Storage \<Rightarrow> coupon_storage l r
+       | Apply \<Rightarrow> coupon_apply l r
+       | Slice \<Rightarrow> coupon_slice l r
+       | Think \<Rightarrow> coupon_think l r
+       | Eval \<Rightarrow> coupon_eval l r
+       | Eq \<Rightarrow> coupon_eq l r)
+   | _ \<Rightarrow> False)"
+
+(* CouponTreeEq *)
+fun make_eq_tree_coupon :: "handle list \<Rightarrow> handle \<Rightarrow> handle \<Rightarrow> handle option" where
+  "make_eq_tree_coupon coupons l r =
+   (if (\<forall>i. (i < length coupons \<longrightarrow> is_eq_coupon (coupons ! i))) then
     (if (get_tree_size_api l = Some (length coupons) \<and> get_tree_size_api r = Some (length coupons)) then
       (if (\<forall>i. (i < length coupons \<longrightarrow>
          (case (get_tree_data_api l i, get_tree_data_api r i, get_coupon_lhs (coupons ! i), get_coupon_rhs (coupons ! i)) of
              (Some li, Some ri, Some cl, Some cr) \<Rightarrow> (is_equal li cl \<and> is_equal ri cr)
            | _ \<Rightarrow> False))) 
-      then Some (create_eq_coupon l r) else None)
+      then Some (create_coupon Eq l r) else None)
     else None)
   else None)"
 
-fun make_thunk_coupon_raw :: "handle list \<Rightarrow> handle \<Rightarrow> handle \<Rightarrow> handle option" where
-  "make_thunk_coupon_raw (f1 # f2 # e # xs) l r =
-   (if ((is_force_coupon_api f1) \<and> (is_force_coupon_api f2) \<and> (is_eq_coupon_api e)) 
+lemma eq_lhs_exist:
+  assumes "is_eq_coupon c"
+  shows "\<exists>l. get_coupon_lhs c = Some l"
+  using assms get_coupon_lhs_match get_coupon_type_exists is_eq_coupon_def by blast
+
+lemma eq_rhs_exist:
+  assumes "is_eq_coupon c"
+  shows "\<exists>r. get_coupon_rhs c = Some r"
+  using assms get_coupon_rhs_match get_coupon_type_exists is_eq_coupon_def by blast
+
+lemma eval_lhs_exist:
+  assumes "is_eval_coupon c"
+  shows "\<exists>l. get_coupon_lhs c = Some l"
+  using assms get_coupon_lhs_match get_coupon_type_exists is_eval_coupon_def by blast
+
+lemma eval_rhs_exist:
+  assumes "is_eval_coupon c"
+  shows "\<exists>r. get_coupon_rhs c = Some r"
+  using assms get_coupon_rhs_match get_coupon_type_exists is_eval_coupon_def by blast
+
+lemma think_lhs_exist:
+  assumes "is_think_coupon c"
+  shows "\<exists>l. get_coupon_lhs c = Some l"
+  using assms get_coupon_lhs_match get_coupon_type_exists is_think_coupon_def by blast
+
+lemma think_rhs_exist:
+  assumes "is_think_coupon c"
+  shows "\<exists>r. get_coupon_rhs c = Some r"
+  using assms get_coupon_rhs_match get_coupon_type_exists is_think_coupon_def by blast
+
+lemma apply_lhs_exist:
+  assumes "is_apply_coupon c"
+  shows "\<exists>l. get_coupon_lhs c = Some l"
+  using assms get_coupon_lhs_match get_coupon_type_exists is_apply_coupon_def by blast
+
+lemma apply_rhs_exist:
+  assumes "is_apply_coupon c"
+  shows "\<exists>r. get_coupon_rhs c = Some r"
+  using assms get_coupon_rhs_match get_coupon_type_exists is_apply_coupon_def by blast
+
+lemma force_lhs_exist:
+  assumes "is_force_coupon c"
+  shows "\<exists>l. get_coupon_lhs c = Some l"
+  using assms get_coupon_lhs_match get_coupon_type_exists is_force_coupon_def by blast
+
+lemma force_rhs_exist:
+  assumes "is_force_coupon c"
+  shows "\<exists>r. get_coupon_rhs c = Some r"
+  using assms get_coupon_rhs_match get_coupon_type_exists is_force_coupon_def by blast
+
+lemma good_eq:
+  assumes "coupon_good c"
+  and "is_eq_coupon c"
+shows "coupon_eq (the (get_coupon_lhs c)) (the (get_coupon_rhs c))"
+  using eq_lhs_exist eq_rhs_exist coupon_good_def
+  apply simp
+  using assms(1,2) is_eq_coupon_def by fastforce
+
+lemma good_eval:
+  assumes "coupon_good c"
+  and "is_eval_coupon c"
+shows "coupon_eval (the (get_coupon_lhs c)) (the (get_coupon_rhs c))"
+  using eval_lhs_exist eval_rhs_exist coupon_good_def
+  apply simp
+  using assms(1,2) is_eval_coupon_def by fastforce
+
+lemma good_apply:
+  assumes "coupon_good c"
+  and "is_apply_coupon c"
+shows "coupon_apply (the (get_coupon_lhs c)) (the (get_coupon_rhs c))"
+  using apply_lhs_exist apply_rhs_exist coupon_good_def
+  apply simp
+  using assms(1,2) is_apply_coupon_def by fastforce
+
+lemma good_force:
+  assumes "coupon_good c"
+  and "is_force_coupon c"
+shows "coupon_force (the (get_coupon_lhs c)) (the (get_coupon_rhs c))"
+  using coupon_good_def is_force_coupon_def get_coupon_type_exists
+  apply simp
+  using assms(1,2) force_lhs_exist force_rhs_exist
+  by force
+
+lemma make_eq_tree_coupon_good:
+  assumes H1: "list_all coupon_good coupons"
+  and H2: "make_eq_tree_coupon coupons l r = Some c"
+shows "coupon_good c"
+proof - 
+  have H: "(\<forall>i. (i < length coupons \<longrightarrow> is_eq_coupon (coupons ! i)))"
+    using H2
+    by (metis make_eq_tree_coupon.simps
+        option.distinct(1))
+
+  then have Sizel: "get_tree_size_api l = Some (length coupons)"
+       and  Sizer: "get_tree_size_api r = Some (length coupons)"
+    using H
+    by (metis H2 make_eq_tree_coupon.simps option.distinct(1))+
+
+  then obtain tl tr where "l = HTreeObj tl" and "r = HTreeObj tr"
+    using HTreeObj_def
+    apply (cases l; cases r; simp_all)
+    by (metis Data.simps(5,6) Object.simps(5) lower_data.cases
+        option.distinct(1))
+
+  then have "(\<forall>i. (i < length coupons \<longrightarrow>
+         (get_tree_data tl i = the (get_coupon_lhs (coupons ! i))) \<and> get_tree_data tr i = the (get_coupon_rhs (coupons ! i))))"
+    using H H2 Sizel Sizer get_tree_size_def get_tree_data_def
+    by (simp, metis (no_types, lifting) is_equal_match
+        option.case_eq_if option.discI)
+
+  then have "(\<forall>i. (i < length coupons \<longrightarrow>
+         (coupon_eq (get_tree_data tl i) (get_tree_data tr i))))"
+    by (metis H H1 good_eq list_all_length)
+  then have "coupon_eq (HTreeObj tl) (HTreeObj tr)"
+    using coupon_force_coupon_storage_coupon_apply_coupon_slice_coupon_identify_coupon_think_coupon_eval_coupon_eq.CouponTreeEq
+get_tree_data_def get_tree_size_def Sizel Sizer
+    by (simp add: \<open>l = HTreeObj tl\<close> \<open>r = HTreeObj tr\<close>
+        list_all2_all_nthI)
+
+  have "c = create_coupon Eq l r"
+    by (metis (no_types, lifting) H2
+        make_eq_tree_coupon.simps option.discI
+        option.inject)
+  then show ?thesis
+    using \<open>coupon_eq (HTreeObj tl) (HTreeObj tr)\<close>
+      \<open>l = HTreeObj tl\<close> \<open>r = HTreeObj tr\<close>
+      coupon_good_def by force
+qed
+
+(* CouponForceResultEq *)
+fun make_force_result_eq_coupon :: "handle list \<Rightarrow> handle \<Rightarrow> handle \<Rightarrow> handle option" where
+  "make_force_result_eq_coupon (f1 # f2 # e # xs) l r =
+   (if ((is_force_coupon f1) \<and> (is_force_coupon f2) \<and> (is_eq_coupon e)) 
     then
      (case (get_coupon_lhs f1, get_coupon_rhs f1, get_coupon_lhs f2, get_coupon_rhs f2,  get_coupon_lhs e, get_coupon_rhs e) of
       (Some f1l, Some f1r, Some f2l, Some f2r, Some el, Some er) \<Rightarrow>
-         (if (is_equal f1r el \<and> is_equal f2r er \<and> is_equal f1l l \<and> is_equal f2l r) then Some (create_eq_coupon l r) else None)
+         (if (is_equal f1r el \<and> is_equal f2r er \<and> is_equal f1l l \<and> is_equal f2l r) then Some (create_coupon Eq l r) else None)
      | _ \<Rightarrow> None)
     else None)"
-| "make_thunk_coupon_raw _ _ _ = None"
+| "make_force_result_eq_coupon _ _ _ = None"
 
-fun make_thunktree_coupon_raw :: "handle list \<Rightarrow> handle \<Rightarrow> handle \<Rightarrow> handle option" where
-  "make_thunktree_coupon_raw (e # xs) l r =
-   (if (is_eq_coupon_api e) then
+lemma make_force_result_eq_coupon_good:
+  assumes H1: "list_all coupon_good coupons"
+  and H2: "make_force_result_eq_coupon coupons l r = Some c"
+shows "coupon_good c"
+proof - 
+  obtain f1 f2 e xs where COUPONS: "coupons = f1 # f2 # e # xs"
+    using H2
+    apply (cases coupons; simp_all)
+    by (metis make_force_result_eq_coupon.simps(3,4) option.distinct(1)
+        remdups_adj.cases)
+
+  then have F1: "is_force_coupon f1" and F2: "is_force_coupon f2" and E: "is_eq_coupon e"
+    using H2
+    by (metis H2 make_force_result_eq_coupon.simps(1) option.distinct(1))+
+
+  moreover then obtain f1l f1r f2l f2r el er 
+    where f1l: "get_coupon_lhs f1 = Some f1l"
+    and   f1r: "get_coupon_rhs f1 = Some f1r"
+    and   f2l: "get_coupon_lhs f2 = Some f2l"
+    and   f2r: "get_coupon_rhs f2 = Some f2r"
+    and   el: "get_coupon_lhs e = Some el"
+    and   er: "get_coupon_rhs e = Some er"
+    using force_lhs_exist force_rhs_exist eq_lhs_exist eq_rhs_exist
+    by presburger
+
+  moreover have "coupon_good f1" 
+           and "coupon_good f2" 
+           and "coupon_good e"
+    using H1
+    by (simp add: \<open>coupons = f1 # f2 # e # xs\<close>)+
+
+  ultimately have "coupon_force f1l f1r"  
+             and "coupon_force f2l f2r" 
+             and "coupon_eq el er"
+    using H1 is_force_coupon_def coupon_good_def good_eq good_force
+    using \<open>coupon_good e\<close> 
+    by (simp_all, fastforce)
+
+  moreover have "f1r = el \<and> f2r = er \<and> f1l = l \<and> f2l = r"
+           and "c = create_coupon Eq l r"
+    using H2 F1 F2 E COUPONS f1l f1r f2l f2r el er
+    by (simp, metis option.distinct(1) option.sel)+
+
+  ultimately show ?thesis
+    using CouponForceResultEq coupon_good_def
+    by simp
+qed
+
+(* CouponThinkApplication *)
+fun make_think_application_coupon :: "handle list \<Rightarrow> handle \<Rightarrow> handle \<Rightarrow> handle option" where
+"make_think_application_coupon (c1 # c2 # xs) l r =
+  (if (is_eval_coupon c1 \<and> is_apply_coupon c2) then
+     (case (get_coupon_lhs c1, get_coupon_rhs c1, get_coupon_lhs c2, get_coupon_rhs c2) of
+       (Some evall, Some evalr, Some applyl, Some applyr) \<Rightarrow>
+         (if (is_equal evalr applyl) then
+           (case (create_application_thunk_api evall) of
+             Some thunk \<Rightarrow>
+               (if (is_equal thunk l \<and> is_equal applyr r) then Some (create_coupon Think l r) else None)
+           | _ \<Rightarrow> None)
+         else None)
+     | _ \<Rightarrow> None)
+   else None)"
+| "make_think_application_coupon _ l r = None"
+
+lemma make_think_application_coupon_good:
+  assumes H1: "list_all coupon_good coupons"
+  and H2: "make_think_application_coupon coupons l r = Some c"
+shows "coupon_good c"
+proof -
+  obtain c1 c2 xs where COUPONS: "coupons = c1 # c2 # xs"
+    using H2
+    by (cases coupons; simp_all; case_tac list; simp_all)
+
+  then have C1: "is_eval_coupon c1" and C2: "is_apply_coupon c2"
+    using H2
+    by (metis make_think_application_coupon.simps(1)
+        option.distinct(1))+
+
+  then obtain c1l c1r c2l c2r
+    where c1l: "get_coupon_lhs c1 = Some c1l"
+    and c1r: "get_coupon_rhs c1 = Some c1r"
+    and c2l: "get_coupon_lhs c2 = Some c2l"
+    and c2r: "get_coupon_rhs c2 = Some c2r"
+    using eval_lhs_exist eval_rhs_exist apply_lhs_exist apply_rhs_exist
+    by presburger
+
+  then have C1C: "coupon_eval c1l c1r" and C2C: "coupon_apply c2l c2r"
+    using C1 C2 COUPONS H1 good_eval good_apply
+    by fastforce+
+
+  obtain thunk where SAME: "c1r = c2l" 
+                        and THUNK: "create_application_thunk_api c1l = Some thunk"
+    using H2 COUPONS C1 C2 c1l c1r c2l c2r
+    apply (simp, meson option.distinct(1))
+    by (metis (lifting) create_application_thunk_api_match
+        option.distinct(1) option.exhaust_sel option.simps(4))
+
+  then obtain c1lt where "c1l = HTreeObj c1lt"
+    using create_application_thunk_api_match HTreeObj_def
+    by (simp, metis (lifting) Data.simps(5,6) Object.simps(5)
+        handle.exhaust handle.simps(10,11,12) lower_data.cases
+        not_Some_eq)
+
+  moreover obtain c2lt where "c2l = HTreeObj c2lt"
+    using C2C coupon_sound
+    by meson
+
+  ultimately have "coupon_think thunk c2r"
+    using CouponThinkApplication
+    C1C C2C SAME THUNK
+    by (simp, blast)
+
+  moreover have "c = create_coupon Think thunk c2r"
+    using H2 C1 C2 C1C C2C COUPONS c1l c1r c2l c2r THUNK SAME
+    by (simp, metis option.distinct(1) option.inject)
+
+  ultimately show ?thesis
+    using coupon_good_def
+    by simp
+qed
+
+(* CouponThinkToForce *)
+fun make_think_to_force_coupon :: "handle list \<Rightarrow> handle \<Rightarrow> handle \<Rightarrow> handle option" where
+"make_think_to_force_coupon (t # xs) l r =
+  (if (is_think_coupon t) then
+    (case (get_coupon_lhs t, get_coupon_rhs t) of
+       (Some l', Some r') \<Rightarrow>
+          (if (get_type r' = 0 \<or> get_type r' = 1 \<or> get_type r' = 2 \<or> get_type r' = 3) then
+            (if (is_equal l' l \<and> is_equal r' r) then
+              Some (create_coupon Force l r)
+            else None)
+          else None)
+     | _ \<Rightarrow> None)
+   else None)"
+| "make_think_to_force_coupon [] l r = None"
+
+lemma make_think_to_force_coupon_good:
+  assumes "list_all coupon_good coupons"
+  and "make_think_to_force_coupon coupons l r = Some c"
+shows "coupon_good c"
+proof -
+  obtain t xs where step1: "coupons = t # xs"
+    using assms(2)
+    by (cases coupons; simp_all)
+
+  then have step2: "is_think_coupon t"
+    using assms(2)
+    by (metis make_think_to_force_coupon.simps(1) option.distinct(1))
+
+  then obtain tl tr where
+        tl: "get_coupon_lhs t = Some tl"
+    and tr: "get_coupon_rhs t = Some tr"
+    using think_lhs_exist think_rhs_exist
+    by presburger
+
+  then have tc: "coupon_think tl tr"
+    using assms(1) step1 step2 coupon_good_def is_think_coupon_def
+    by simp
+
+  have "get_type tr = 0 \<or> get_type tr = 1 \<or> get_type tr = 2 \<or> get_type tr = 3"
+  and "tl = l \<and> tr = r"
+  and "c = create_coupon Force l r"
+    using step1 step2 assms(2) tl tr
+    apply (simp, meson option.distinct(1))
+    using step1 step2 assms(2) tl tr
+    apply (simp, meson is_equal_match
+        option.distinct(1))
+    using step1 step2 assms(2) tl tr
+    by (simp, metis not_Some_eq option.inject)
+
+  then obtain d where "tr = Data d"
+    by (cases tr; force)
+
+  then have "coupon_force tl tr"
+    using tc
+    by (metis CouponThinktoForce
+        coupon_sound)
+
+  then show ?thesis
+    using coupon_good_def
+    by (simp add: \<open>c = create_coupon Force l r\<close>
+        \<open>tl = l \<and> tr = r\<close>)
+qed
+
+(* CouponEqApplication *)
+fun make_eq_application_coupon :: "handle list \<Rightarrow> handle \<Rightarrow> handle \<Rightarrow> handle option" where
+  "make_eq_application_coupon (e # xs) l r =
+   (if (is_eq_coupon e) then
       (case (get_coupon_lhs e, get_coupon_rhs e) of
        (Some l', Some r') \<Rightarrow> 
-         (case (create_thunk_api l', create_thunk_api r') of
+         (case (create_application_thunk_api l', create_application_thunk_api r') of
            (Some l'', Some r'') \<Rightarrow> 
-           (if (is_equal l l'' \<and> is_equal r r'') then Some(create_eq_coupon l r) else None)
+           (if (is_equal l l'' \<and> is_equal r r'') then Some(create_coupon Eq l r) else None)
           | _ \<Rightarrow> None)
        | _ \<Rightarrow> None)
      else None)"
-| "make_thunktree_coupon_raw [] l r = None"
+| "make_eq_application_coupon [] l r = None"
 
-fun make_thunkforce_coupon_raw :: "handle list \<Rightarrow> handle \<Rightarrow> handle \<Rightarrow> handle option" where
-"make_thunkforce_coupon_raw (e # f1 # f2 # xs) l r = 
-   (if ((is_eq_coupon_api e) \<and> (is_force_coupon_api f1) \<and> (is_force_coupon_api f2))
-    then
-    (case (get_coupon_lhs e, get_coupon_rhs e, get_coupon_lhs f1, get_coupon_rhs f1, get_coupon_lhs f2, get_coupon_rhs f2) of
-     (Some el, Some er, Some f1l, Some f1r, Some f2l, Some f2r) \<Rightarrow>
-        (if (is_equal f1l el \<and> is_equal f2l er \<and> is_equal f1r l \<and> is_equal f2r r) then
-         Some (create_eq_coupon l r)
-        else None)
+lemma make_eq_application_coupon_good:
+  assumes "list_all coupon_good coupons"
+  and "make_eq_application_coupon coupons l r = Some c"
+shows "coupon_good c"
+proof - 
+  obtain e xs where step1: "coupons = e # xs"
+    using assms(2)
+    by (cases coupons; simp_all)
+
+  then have step2: "is_eq_coupon e" 
+    using assms(2)
+    by (metis make_eq_application_coupon.simps(1)
+        option.distinct(1))
+
+  then obtain el er where el: "get_coupon_lhs e = Some el"
+                    and   er: "get_coupon_rhs e = Some er"
+    using eq_lhs_exist eq_rhs_exist
+    by blast
+
+  then obtain l' r' where l': "create_application_thunk_api el = Some l'"
+                    and   r': "create_application_thunk_api er = Some r'"
+    using step1 step2 assms(2)
+    by (simp, metis (no_types, lifting) option.case_eq_if
+        option.exhaust_sel)
+
+  then obtain treel treer where treel: "el = HTreeObj treel" 
+                          and treer: "er = HTreeObj treer"
+    using create_application_thunk_api_match
+    by (simp_all, metis (lifting) Data.exhaust Data.simps(5,6)
+        Object.exhaust Object.simps(5) handle.exhaust
+        handle.simps(10,11,12)
+        option.distinct(1))
+
+  have "l' = l" and "r' = r" and "c = create_coupon Eq l' r'"
+    using step1 step2 assms(2) el er l' r' is_equal_match
+    by (simp_all, metis option.distinct(1) option.sel)+
+
+  have "coupon_eq el er"
+    using el er step1 step2 assms(1) good_eq by force
+  then have "coupon_eq l' r'"
+    using l' r' create_application_thunk_api_match treel treer
+    using CouponEqApplication by auto
+  then show ?thesis
+    by (simp add: \<open>c = create_coupon Eq l' r'\<close>
+        coupon_good_def)
+qed
+
+(* CouponEvalBlobObj *)
+fun make_eval_blob_coupon :: "handle list \<Rightarrow> handle \<Rightarrow> handle \<Rightarrow> handle option" where
+"make_eval_blob_coupon _ l r =
+   (if (get_type l = 0 \<and> is_equal l r) then
+     Some (create_coupon Eval l r)
+   else None)"
+
+lemma make_eval_blob_coupon_good:
+  assumes "make_eval_blob_coupon coupons l r = Some c"
+  shows "coupon_good c"
+proof -
+  have step1: "get_type l = 0 \<and> is_equal l r"
+    using assms
+    by (simp, meson option.distinct(1))
+
+  then have "c = create_coupon Eval l r"
+    using assms
+    by auto
+
+  moreover obtain b where "l = HBlobObj b"
+    using step1 HBlobObj_def
+    apply (cases l; simp_all; case_tac x1; simp_all)
+    apply (metis Object.exhaust get_type.simps(2)
+        zero_neq_one)
+    by (metis Ref.exhaust Suc_1 eval_nat_numeral(3)
+        get_type.simps(3,4) old.nat.distinct(1))
+
+  ultimately show ?thesis
+    using coupon_good_def step1 CouponEvalBlobObj
+    by (simp, blast)
+qed
+
+(* CouponEvalTreeObj *)
+fun make_eval_tree_coupon :: "handle list \<Rightarrow> handle \<Rightarrow> handle \<Rightarrow> handle option" where
+  "make_eval_tree_coupon coupons l r =
+   (if (\<forall>i. (i < length coupons \<longrightarrow> is_eval_coupon (coupons ! i))) then
+    (if (get_tree_size_api l = Some (length coupons) \<and> get_tree_size_api r = Some (length coupons)) then
+      (if (\<forall>i. (i < length coupons \<longrightarrow>
+         (case (get_tree_data_api l i, get_tree_data_api r i, get_coupon_lhs (coupons ! i), get_coupon_rhs (coupons ! i)) of
+             (Some li, Some ri, Some cl, Some cr) \<Rightarrow> (is_equal li cl \<and> is_equal ri cr)
+           | _ \<Rightarrow> False))) 
+      then Some (create_coupon Eval l r) else None)
+    else None)
+  else None)"
+
+lemma make_eval_tree_coupon_good:
+  assumes H1: "list_all coupon_good coupons"
+  and H2: "make_eval_tree_coupon coupons l r = Some c"
+shows "coupon_good c"
+proof - 
+  have H: "(\<forall>i. (i < length coupons \<longrightarrow> is_eval_coupon (coupons ! i)))"
+    using H2
+    by (metis make_eval_tree_coupon.simps
+        option.distinct(1))
+
+  then have Sizel: "get_tree_size_api l = Some (length coupons)"
+       and  Sizer: "get_tree_size_api r = Some (length coupons)"
+    using H
+    by (metis H2 make_eval_tree_coupon.simps option.distinct(1))+
+
+  then obtain tl tr where "l = HTreeObj tl" and "r = HTreeObj tr"
+    using HTreeObj_def
+    apply (cases l; cases r; simp_all)
+    by (metis Data.simps(5,6) Object.simps(5) lower_data.cases
+        option.distinct(1))
+
+  then have "(\<forall>i. (i < length coupons \<longrightarrow>
+         (get_tree_data tl i = the (get_coupon_lhs (coupons ! i))) \<and> get_tree_data tr i = the (get_coupon_rhs (coupons ! i))))"
+    using H H2 Sizel Sizer get_tree_size_def get_tree_data_def
+    by (simp, metis (no_types, lifting) is_equal_match
+        option.case_eq_if option.discI)
+
+  then have "(\<forall>i. (i < length coupons \<longrightarrow>
+         (coupon_eval (get_tree_data tl i) (get_tree_data tr i))))"
+    by (metis H H1 good_eval list_all_length)
+  then have "coupon_eval (HTreeObj tl) (HTreeObj tr)"
+    using CouponEvalTreeObj get_tree_data_def get_tree_size_def Sizel Sizer
+    by (simp add: \<open>l = HTreeObj tl\<close> \<open>r = HTreeObj tr\<close>
+        list_all2_all_nthI)
+
+  have "c = create_coupon Eval l r"
+    by (metis (no_types, lifting) H2
+        make_eval_tree_coupon.simps option.discI
+        option.inject)
+  then show ?thesis
+    using \<open>coupon_eval (HTreeObj tl) (HTreeObj tr)\<close>
+      \<open>l = HTreeObj tl\<close> \<open>r = HTreeObj tr\<close>
+      coupon_good_def by force
+qed
+
+(* CouponForcetoEncodeStrict *)
+fun make_force_to_encode_strict_coupon :: "handle list \<Rightarrow> handle \<Rightarrow> handle \<Rightarrow> handle option"
+where 
+"make_force_to_encode_strict_coupon (e # xs) l r = 
+  (if (is_force_coupon e) then
+    (case (get_coupon_lhs e, get_coupon_rhs e) of
+      (Some el, Some er) \<Rightarrow>
+         (case (create_strict_encode_api el) of
+           Some el' \<Rightarrow> 
+            (if (is_equal el' l \<and> is_equal er r \<and> (get_type er = 0 
+                                                 \<or> get_type er = 1)) 
+              then Some (create_coupon Eq l r)
+              else None)
+         | None \<Rightarrow> None)
      | _ \<Rightarrow> None)
    else None)"
-| "make_thunkforce_coupon_raw _ l r = None"
+| "make_force_to_encode_strict_coupon [] l r = None"
 
-fun make_encode_coupon_raw :: "handle list \<Rightarrow> handle \<Rightarrow> handle \<Rightarrow> handle option" where
- "make_encode_coupon_raw (e # xs) l r =
-  (if (is_eq_coupon_api e) then
+lemma make_force_to_encode_strict_coupon_good:
+  assumes "list_all coupon_good coupons"
+  and "make_force_to_encode_strict_coupon coupons l r = Some c"
+shows "coupon_good c"
+proof -
+  obtain e xs where step1: "coupons = e # xs"
+    using assms(2)
+    by (cases coupons; simp_all)
+
+  then have step2: "is_force_coupon e"
+    using assms(2)
+    by (simp, metis option.discI)
+
+  then obtain el er where el: "get_coupon_lhs e = Some el"
+                    and   er: "get_coupon_rhs e = Some er"
+    using force_lhs_exist force_rhs_exist
+    by blast
+
+  then obtain el' where el': "create_strict_encode_api el = Some el'"
+    using assms(2) step1 step2 el er
+    by (simp, fastforce)
+
+  then have step3: "(is_equal el' l \<and> is_equal er r \<and> (get_type er = 0 
+                                                 \<or> get_type er = 1))"
+    using assms(2) step1 step2 el er
+    by (simp, metis option.distinct(1))
+  then have step4: "c = create_coupon Eq l r"
+    using assms(2) step1 step2 el er el' 
+    by (simp, force)
+
+  have "coupon_force el er"
+    using step2 assms(2) step1 el er
+    using assms(1) good_force by fastforce
+  moreover have "lift er = er"
+    using step3 
+    apply (cases er; simp_all)
+    apply (case_tac x1; simp_all)
+    apply force
+    by (case_tac x2; simp_all)
+  ultimately have "coupon_eq el' er"
+    using el' create_strict_encode_api_match CouponForcetoEncodeStrict
+    apply simp
+    apply (cases el; simp_all)
+    by fastforce
+
+  then show ?thesis
+    using coupon_good_def step4 step3
+    by simp
+qed
+
+(* CouponEvalEq *)
+fun make_eval_eq_coupon :: "handle list \<Rightarrow> handle \<Rightarrow> handle \<Rightarrow> handle option"
+  where
+"make_eval_eq_coupon (c1 # c2 # xs) l r =
+ (if (is_eval_coupon c1 \<and> is_eq_coupon c2) then
+    (case (get_coupon_lhs c1, get_coupon_rhs c1, get_coupon_lhs c2, get_coupon_rhs c2) of
+    (Some evall, Some evalr, Some eql, Some eqr) \<Rightarrow>
+       (if (is_equal evall eql \<and> is_equal eqr l \<and> is_equal evalr r) then
+          Some (create_coupon Eval l r)
+        else None)
+  | _ \<Rightarrow> None)
+ else None)"
+| "make_eval_eq_coupon _ l r = None"
+
+lemma make_eval_eq_coupon_good:
+  assumes "list_all coupon_good coupons"
+and "make_eval_eq_coupon coupons l r = Some c"
+shows "coupon_good c"
+proof -
+  obtain c1 c2 xs where step1: "coupons = c1 # c2 # xs"
+    using assms(2)
+    by (cases coupons; simp_all; case_tac list; simp_all)
+
+  then have step2: "is_eval_coupon c1 \<and> is_eq_coupon c2"
+    using assms(2)
+    by (metis make_eval_eq_coupon.simps(1)
+        option.distinct(1))
+
+  then obtain c1l c1r c2l c2r 
+    where c1l: "get_coupon_lhs c1 = Some c1l"
+    and   c1r: "get_coupon_rhs c1 = Some c1r"
+    and   c2l: "get_coupon_lhs c2 = Some c2l"
+    and   c2r: "get_coupon_rhs c2 = Some c2r"
+    using eval_lhs_exist eval_rhs_exist eq_lhs_exist eq_rhs_exist
+    by presburger
+
+  then have step3: "is_equal c1l c2l \<and> is_equal c2r l \<and> is_equal c1r r"
+    using assms(2) step1 step2
+    by (simp, metis option.distinct(1))
+  then have step4: "c = create_coupon Eval l r"
+    using assms(2) step1 step2 c1l c1r c2l c2r
+    by simp
+
+  have "coupon_eval c1l c1r"
+    using step2 step1 coupon_good_def assms(1) c1l c1r good_eval by force
+  moreover have "coupon_eq c1l c2r"
+    using step2 step1 coupon_good_def assms(1) c2l c2r good_eq step3 by force
+  ultimately have "coupon_eval c2r c1r"
+    using CouponEvalEq by blast
+  then show ?thesis 
+    using step1 step4 step3 coupon_good_def
+    by auto
+qed
+
+(* CouponEqEncodeStrict *)
+fun make_eq_encode_strict_coupon :: "handle list \<Rightarrow> handle \<Rightarrow> handle \<Rightarrow> handle option" where
+ "make_eq_encode_strict_coupon (e # xs) l r =
+  (if (is_eq_coupon e) then
     (case (get_coupon_lhs e, get_coupon_rhs e) of
       (Some l', Some r') \<Rightarrow>
-       (case (create_encode_api l', create_encode_api r') of
+       (case (create_strict_encode_api l', create_strict_encode_api r') of
          (Some l'', Some r'') \<Rightarrow>
-           (if (is_equal l l'' \<and> is_equal r r'') then Some (create_eq_coupon l r) else None)
+           (if (is_equal l l'' \<and> is_equal r r'') then Some (create_coupon Eq l r) else None)
         | _ \<Rightarrow> None)
       | _ \<Rightarrow> None)
     else None)"
-| "make_encode_coupon_raw [] l r = None"
+| "make_eq_encode_strict_coupon [] l r = None"
 
-fun make_sym_coupon_raw :: "handle list \<Rightarrow> handle \<Rightarrow> handle \<Rightarrow> handle option" where
-  "make_sym_coupon_raw (e # xs) l r =
-   (if (is_eq_coupon_api e) then
+lemma make_eq_encode_strict_coupon_good:
+  assumes "list_all coupon_good coupons"
+  and "make_eq_encode_strict_coupon coupons l r = Some c"
+shows "coupon_good c"
+proof -
+  obtain e xs where step1: "coupons = e # xs"
+    using assms(2)
+    by (cases coupons; simp_all)
+
+  then have step2: "is_eq_coupon e"
+    using assms(2)
+    by (simp, metis option.discI)
+
+  then obtain el er where el: "get_coupon_lhs e = Some el"
+                    and   er: "get_coupon_rhs e = Some er"
+    using eq_lhs_exist eq_rhs_exist
+    by blast
+
+  then obtain el' er' where el': "create_strict_encode_api el = Some el'"
+                      and   er': "create_strict_encode_api er = Some er'"
+    using assms(2) step1 step2
+    apply simp
+    by (metis (no_types, lifting) option.case_eq_if
+        option.exhaust)
+
+  then have step3: "l = el' \<and> r = er'" and step4: "c = create_coupon Eq l r"
+    using assms(2) step1 step2 el er
+    apply simp_all
+    apply (metis option.distinct(1))
+    by (metis option.distinct(1) option.sel)
+
+  have "coupon_eq el er"
+    using step2 assms(1) coupon_good_def step1 el er
+    using good_eq by force
+  have "coupon_eq el' er'"
+    using el' er' create_strict_encode_api_match CouponEqEncodeStrict
+    apply (cases el; cases er; simp_all)
+    using \<open>coupon_eq el er\<close> by blast
+  then show ?thesis
+    using step4 coupon_good_def step3
+    by simp
+qed
+
+(* CouponEqEncodeShallow *)
+fun make_eq_encode_shallow_coupon :: "handle list \<Rightarrow> handle \<Rightarrow> handle \<Rightarrow> handle option" where
+ "make_eq_encode_shallow_coupon (e # xs) l r =
+  (if (is_eq_coupon e) then
+    (case (get_coupon_lhs e, get_coupon_rhs e) of
+      (Some l', Some r') \<Rightarrow>
+       (case (create_shallow_encode_api l', create_shallow_encode_api r') of
+         (Some l'', Some r'') \<Rightarrow>
+           (if (is_equal l l'' \<and> is_equal r r'') then Some (create_coupon Eq l r) else None)
+        | _ \<Rightarrow> None)
+      | _ \<Rightarrow> None)
+    else None)"
+| "make_eq_encode_shallow_coupon [] l r = None"
+
+lemma make_eq_encode_shallow_coupon_good:
+  assumes "list_all coupon_good coupons"
+  and "make_eq_encode_shallow_coupon coupons l r = Some c"
+shows "coupon_good c"
+proof -
+  obtain e xs where step1: "coupons = e # xs"
+    using assms(2)
+    by (cases coupons; simp_all)
+
+  then have step2: "is_eq_coupon e"
+    using assms(2)
+    by (simp, metis option.discI)
+
+  then obtain el er where el: "get_coupon_lhs e = Some el"
+                    and   er: "get_coupon_rhs e = Some er"
+    using eq_lhs_exist eq_rhs_exist
+    by blast
+
+  then obtain el' er' where el': "create_shallow_encode_api el = Some el'"
+                      and   er': "create_shallow_encode_api er = Some er'"
+    using assms(2) step1 step2
+    apply simp
+    by (metis (no_types, lifting) option.case_eq_if
+        option.exhaust)
+
+  then have step3: "l = el' \<and> r = er'" and step4: "c = create_coupon Eq l r"
+    using assms(2) step1 step2 el er
+    apply simp_all
+    apply (metis option.distinct(1))
+    by (metis option.distinct(1) option.sel)
+
+  have "coupon_eq el er"
+    using step2 assms(1) coupon_good_def step1 el er
+    using good_eq by force
+  have "coupon_eq el' er'"
+    using el' er' create_shallow_encode_api_match CouponEqEncodeShallow
+    apply (cases el; cases er; simp_all)
+    using \<open>coupon_eq el er\<close> by blast
+  then show ?thesis
+    using step4 coupon_good_def step3
+    by simp
+qed
+
+(* CouponSym *)
+fun make_sym_coupon :: "handle list \<Rightarrow> handle \<Rightarrow> handle \<Rightarrow> handle option" where
+  "make_sym_coupon (e # xs) l r =
+   (if (is_eq_coupon e) then
      (case (get_coupon_lhs e, get_coupon_rhs e) of
       (Some l', Some r') \<Rightarrow>
-        (if (is_equal r' l \<and> is_equal l' r) then Some (create_eq_coupon l r) else None)
+        (if (is_equal r' l \<and> is_equal l' r) then Some (create_coupon Eq l r) else None)
       | _ \<Rightarrow> None)
    else None)"
-| "make_sym_coupon_raw _ l r = None"
+| "make_sym_coupon _ l r = None"
 
-fun make_trans_coupon_raw :: "handle list \<Rightarrow> handle \<Rightarrow> handle \<Rightarrow> handle option" where
- "make_trans_coupon_raw (e1 # e2 # xs) l r = 
-    (if (is_eq_coupon_api e1 \<and> is_eq_coupon_api e2) then
+lemma make_sym_coupon_good:
+  assumes "list_all coupon_good coupons"
+and "make_sym_coupon coupons l r = Some c"
+shows "coupon_good c"
+proof -
+  obtain e xs where step1: "coupons = e # xs"
+    using assms(2)
+    by (cases coupons; simp_all)
+
+  then have step2: "is_eq_coupon e"
+    using assms(2)
+    by (simp, metis option.discI)
+
+  then obtain el er where el: "get_coupon_lhs e = Some el"
+                    and   er: "get_coupon_rhs e = Some er"
+    using eq_lhs_exist eq_rhs_exist
+    by blast
+
+  then have step3: "er = l \<and> el = r"
+    using assms(2) step1 step2
+    by (simp, metis option.distinct(1))
+
+  then have step4: "c = create_coupon Eq l r"
+    using assms(2) step1 step2 el er
+    by simp
+
+  have "coupon_eq el er" 
+    using step2 el er step1 assms(2)
+    using assms(1) good_eq by force
+  then have "coupon_eq l r"
+    using step3 CouponSym
+    by blast
+  then show ?thesis
+    using coupon_good_def step4 by simp
+qed
+
+(* CouponTrans *)
+fun make_trans_coupon :: "handle list \<Rightarrow> handle \<Rightarrow> handle \<Rightarrow> handle option" where
+ "make_trans_coupon (e1 # e2 # xs) l r = 
+    (if (is_eq_coupon e1 \<and> is_eq_coupon e2) then
         (case (get_coupon_lhs e1, get_coupon_rhs e1, get_coupon_lhs e2, get_coupon_rhs e2) of
            (Some e1l, Some e1r, Some e2l, Some e2r) \<Rightarrow>
              (if (is_equal e1r e2l \<and> is_equal l e1l \<and> is_equal r e2r) then
-               Some (create_eq_coupon l r)
+               Some (create_coupon Eq l r)
               else None)
           | _ \<Rightarrow> None)
         else None)"
-| "make_trans_coupon_raw _ l r = None"
-  
+| "make_trans_coupon _ l r = None"
 
-fun make_self_coupon_raw :: "handle list \<Rightarrow> handle \<Rightarrow> handle \<Rightarrow> handle option" where
-"make_self_coupon_raw xs l r = 
+lemma make_trans_coupon_good:
+  assumes "list_all coupon_good coupons"
+  and "make_trans_coupon coupons l r = Some c"
+shows "coupon_good c"
+proof -
+  obtain c1 c2 xs where step1: "coupons = c1 # c2 # xs"
+    using assms(2)
+    by (cases coupons; simp_all; case_tac list; simp_all)
+
+  then have step2: "is_eq_coupon c1 \<and> is_eq_coupon c2"
+    using assms(2)
+    by (metis make_trans_coupon.simps(1)
+        option.distinct(1))
+
+  then obtain c1l c1r c2l c2r 
+    where c1l: "get_coupon_lhs c1 = Some c1l"
+    and   c1r: "get_coupon_rhs c1 = Some c1r"
+    and   c2l: "get_coupon_lhs c2 = Some c2l"
+    and   c2r: "get_coupon_rhs c2 = Some c2r"
+    using eq_lhs_exist eq_rhs_exist
+    by presburger
+
+  then have step3: "is_equal c1r c2l \<and> is_equal l c1l \<and> is_equal r c2r"
+    using assms(2) step1 step2
+    by (simp, metis option.distinct(1))
+
+  then have step4: "c = create_coupon Eq l r"
+    using assms(2) step1 step2 c1l c1r c2l c2r
+    by simp
+
+  have "coupon_eq c1l c1r"
+    using step2 step1 assms(1) coupon_good_def good_eq c1l c1r
+    by force
+  moreover have "coupon_eq c2l c2r"
+    using step2 step1 assms(1) coupon_good_def good_eq c2l c2r
+    by force
+  ultimately have "coupon_eq c1l c2r"
+    by (metis CouponTrans is_equal_match
+        step3)
+  then show ?thesis
+    using step3 coupon_good_def step4
+    by simp
+qed
+
+(* CouponSelf *)
+fun make_self_coupon :: "handle list \<Rightarrow> handle \<Rightarrow> handle \<Rightarrow> handle option" where
+"make_self_coupon _ l r = 
  (if (is_equal l r) then 
-    Some (create_eq_coupon l r) 
+    Some (create_coupon Eq l r) 
   else 
     None)"
 
+lemma make_self_coupon_good:
+  assumes "make_self_coupon coupons l r = Some c"
+  shows "coupon_good c"
+proof -
+  have "is_equal l r"
+    using assms
+    by (metis make_self_coupon.simps
+        option.distinct(1))
+  then have "c = create_coupon Eq l r"
+    using assms
+    by simp
+
+  moreover have "coupon_eq l r"
+    using CouponSelf \<open>is_equal l r\<close>
+    by fastforce
+  ultimately show ?thesis
+    using coupon_good_def
+    by force
+qed
+
 datatype request =
-  Storage | Tree | Thunk | ThunkTree | ThunkForce | Encode | Sym | Trans | Self
+  TreeEq | ForceResultEq | ThinkApplication | ThinkToForce | EqApplication | EvalBlobObj | EvalTreeObj | ForceToEncodeStrict | EvalEq | EqEncodeStrict | Sym | Trans | Self
 
 fun make_coupon :: "request \<Rightarrow> handle list \<Rightarrow> handle \<Rightarrow> handle \<Rightarrow> handle option" where
-  "make_coupon Storage coupons l r = make_storage_coupon_raw coupons l r"
-| "make_coupon Tree coupons l r = make_tree_coupon_raw coupons l r"
-| "make_coupon Thunk coupons l r = make_thunk_coupon_raw coupons l r"
-| "make_coupon ThunkTree coupons l r = make_thunktree_coupon_raw coupons l r"
-| "make_coupon ThunkForce coupons l r = make_thunkforce_coupon_raw coupons l r"
-| "make_coupon Encode coupons l r = make_encode_coupon_raw coupons l r"
-| "make_coupon Self coupons l r = make_self_coupon_raw coupons l r"
-| "make_coupon Sym coupons l r = make_sym_coupon_raw coupons l r"
-| "make_coupon Trans coupons l r = make_trans_coupon_raw coupons l r"
+  "make_coupon TreeEq coupons l r = make_eq_tree_coupon coupons l r"
+| "make_coupon ForceResultEq coupons l r = make_force_result_eq_coupon coupons l r"
+| "make_coupon ThinkApplication coupons l r = make_think_application_coupon coupons l r"
+| "make_coupon ThinkToForce coupons l r = make_think_to_force_coupon coupons l r"
+| "make_coupon EqApplication coupons l r = make_eq_application_coupon coupons l r"
+| "make_coupon EvalBlobObj coupons l r = make_eval_blob_coupon coupons l r"
+| "make_coupon EvalTreeObj coupons l r = make_eval_tree_coupon coupons l r"
+| "make_coupon ForceToEncodeStrict coupons l r = make_force_to_encode_strict_coupon coupons l r"
+| "make_coupon EvalEq coupons l r = make_eval_eq_coupon coupons l r"
+| "make_coupon EqEncodeStrict coupons l r = make_eq_encode_strict_coupon coupons l r"
+| "make_coupon Self coupons l r = make_self_coupon coupons l r"
+| "make_coupon Sym coupons l r = make_sym_coupon coupons l r"
+| "make_coupon Trans coupons l r = make_trans_coupon coupons l r"
+
+lemma make_coupon_good:
+  assumes H1: "list_all coupon_good coupons"
+  and H2: "make_coupon req coupons l r = Some c"
+shows "coupon_good c"
+  using assms(2)
+proof (cases req)
+  case TreeEq
+  then show ?thesis
+    using H1 H2 make_eq_tree_coupon_good
+    by auto
+next
+  case ForceResultEq
+  then show ?thesis
+    using H1 H2 make_force_result_eq_coupon_good
+    by force
+next
+  case ThinkApplication
+  then show ?thesis
+    using H1 H2 make_think_application_coupon_good
+    by force
+next
+  case ThinkToForce
+  then show ?thesis
+    using H1 H2 make_think_to_force_coupon_good
+    by force
+next
+  case EqApplication
+  then show ?thesis
+    using H1 H2 make_eq_application_coupon_good
+    by force
+next
+  case EvalBlobObj
+  then show ?thesis
+    using H2 make_eval_blob_coupon_good
+    by force
+next
+  case EvalTreeObj
+  then show ?thesis
+    using H1 H2 make_eval_tree_coupon_good
+    by force
+next
+  case ForceToEncodeStrict
+  then show ?thesis
+    using H1 H2
+      make_force_to_encode_strict_coupon_good
+    by auto
+next
+  case EvalEq
+  then show ?thesis
+    using H1 H2 make_eval_eq_coupon_good
+    by force
+next
+  case EqEncodeStrict
+  then show ?thesis
+    using H1 H2 make_eq_encode_strict_coupon_good
+    by auto
+next
+  case Sym
+  then show ?thesis
+    using H1 H2 make_sym_coupon_good by force
+next
+  case Trans
+  then show ?thesis
+    using H1 H2 make_trans_coupon_good by force
+next
+  case Self
+  then show ?thesis
+    using H2 make_self_coupon_good by force
+qed
 
 end
